theories/interop/wrappersem.v
@@ -1,5 +1,8 @@
 From stdpp Require Import base strings list gmap.
 From melocoton Require Import multirelations.
+From melocoton.c_toy_lang Require Import lang_instantiation.
+From melocoton.language Require Import language.
+From melocoton.c_toy_lang Require Import lang.
 From melocoton.interop Require Import assums basics wrapperstate.
 
 Inductive ml_or_c (A B: Type) : Type :=
@@ -10,69 +13,106 @@ Arguments ML {A B}.
 Arguments C {A B}.
 
 Section wrappersem.
-Context {WPms: WrapperParameters}.
 
-Definition stateW : Type :=
-  (* state of the wrapper, which depends on whether we are yielding control to
-     ML or executing the wrapped C program. *)
-  ml_or_c
-    (wrapstateML * store)
-    (wrapstateC * memory).
+Inductive wrapper_func_kind : Type :=
+  FuncInternal | FuncExternal.
 
-Definition func : Type := string.
+Definition func : Type :=
+  wrapper_func_kind * C_lang.function.
 
 (* the wrapped C program accepts incoming function calls with ML values as
    arguments, and produces an ML value as output. *)
 (* we don't have callbacks yet, so there's no "make an external call"
    expression: the wrapped C program can only be called into, not make "external
    calls" to ML yet. *)
-Inductive exprW : Type :=
-  | ValW (v : val)
-  | RunningW (ec : exprC)
-  | CallFunctionW (fn : func) (vs : list val).
+Inductive expr : Type :=
+  | WrapExprV (v : val)
+  | WrapExprCall (fn_name : string) (args : list val)
+  | WrapRunExternalFunction (fn : C_lang.function) (args : list val)
+  | WrapExprC (ec : C_lang.expr).
+
+Definition apply_func (fn : func) (args : list val) : option expr :=
+  let '(fnkind, fn) := fn in
+  match fnkind with
+  | FuncInternal => None
+  | FuncExternal => Some (WrapRunExternalFunction fn args)
+  end.
+
+Definition of_class (c : mixin_expr_class val) : expr :=
+  match c with
+  | ExprVal v => WrapExprV v
+  | ExprCall fn_name args => WrapExprCall fn_name args
+  end.
+
+Definition to_class (e : expr) : option (mixin_expr_class val) :=
+  match e with
+  | WrapExprV v => Some (ExprVal v)
+  | WrapExprCall fn_name args => Some (ExprCall fn_name args)
+  | _ => None
+  end.
 
 (* wrapper evaluation contexts should become nontrivial when we add callbacks *)
-Definition ectxW : Type := unit.
-Definition fillW : ectxW → exprW → exprW := λ _ e, e.
+Definition ectx : Type := unit.
+Definition fill : ectx → expr → expr := λ _ e, e.
 
-Definition apply_func (fn : func) (vs : list val) : exprW :=
-  CallFunctionW fn vs.
+Definition state : Type :=
+  (* state of the wrapper, which depends on whether we are yielding control to
+     ML or executing the wrapped C program. *)
+  ml_or_c
+    (wrapstateML * store)
+    (wrapstateC * memory).
 
-Definition wrapper_step (prog : progC) : mrel (exprW * stateW) (exprW * stateW) :=
+Definition private_state : Type :=
+  (* without callbacks we only need ML-related private state *)
+  wrapstateML.
+
+Local Notation prog := (gmap string func).
+
+Definition proj_prog_C (P : prog) : gmap string C_lang.function :=
+  fmap (λ '(_, fn), fn) P.
+
+Definition wrapper_step (P : prog) : mrel (expr * state) (expr * state) :=
   λ '(e, ρ) φ,
     (* step in the underlying wrapped C program *)
     (∀ ec ρc mem ec' mem',
-       e = RunningW ec →
+       e = WrapExprC ec →
        ρ = C (ρc, mem) →
-       head_step_C prog ec mem ec' mem' →
-       φ (RunningW ec', C (ρc, mem')))
+       C_lang.head_step (proj_prog_C P) ec mem ec' mem' →
+       φ (WrapExprC ec', C (ρc, mem')))
+    ∨
+    (* administrative step for resolving a call from ML *)
+    (∀ fn_name args fn,
+       e = WrapExprCall fn_name args →
+       P !! fn_name = Some (FuncExternal, fn) →
+       φ (WrapRunExternalFunction fn args, ρ))
     ∨
     (* incoming call of a C function from ML *)
     (∀ fn vs ρml σ,
-       e = CallFunctionW fn vs →
+       e = WrapRunExternalFunction fn vs →
        ρ = ML (ρml, σ) →
        ∃ χ ζ privσ lvs,
          is_store χ ζ privσ σ ∧
          ML_change_lstore (χML ρml) (ζML ρml) ζ ∧
          ML_extends_lloc_map (ζML ρml) (χML ρml) χ ∧
          Forall2 (is_val χ ζ) vs lvs ∧
-         ∀ ws mem ρc,
+         ∀ ws ec mem ρc,
            (∀ γ (a:addr) v,
               (rootsML ρml) !! a = Some v →
               reachable ζ [v] γ →
               γ ∈ dom (θC ρc)) →
            Forall2 (repr_lval (θC ρc)) lvs ws →
+           C_lang.apply_function fn ws = Some ec →
            repr (θC ρc) (rootsML ρml) (privmemML ρml) mem →
            χC ρc = χ →
            ζC ρc = ζ →
            rootsC ρc = dom (rootsML ρml) →
            privσC ρc = privσ →
-           φ (RunningW (apply_func_C fn ws), C (ρc, mem)))
+           φ (WrapExprC ec, C (ρc, mem)))
     ∨
     (* wrapped C function returning to ML *)
     (∀ ec w ρc mem,
-       e = RunningW ec →
-       to_val_C ec = Some w →
+       e = WrapExprC ec →
+       C_lang.to_val ec = Some w →
        ρ = C (ρc, mem) →
        ∃ σ lv v ρml,
          freeze_lstore (ζC ρc) (ζML ρml) ∧
@@ -82,12 +122,12 @@ Definition wrapper_step (prog : progC) : mrel (exprW * stateW) (exprW * stateW) 
          is_val (χML ρml) (ζML ρml) v lv ∧
          dom (rootsML ρml) = rootsC ρc ∧
          repr (θC ρc) (rootsML ρml) (privmemML ρml) mem ∧
-         φ (ValW v, ML (ρml, σ)))
+         φ (WrapExprV v, ML (ρml, σ)))
     ∨
     (* call from C to the "alloc" primitive *)
     (∀ K ec tgnum tg sz ρc mem,
-       e = RunningW (fillC K ec) →
-       to_call_C ec = Some ("alloc", [tgnum; sz]) →
+       e = WrapExprC (language.fill K ec) →
+       to_call ec = Some ("alloc", [LitV (LitInt tgnum); LitV (LitInt sz)]) →
        ρ = C (ρc, mem) →
        tgnum = tag_as_int tg →
        (0 < sz)%Z →
@@ -106,40 +146,40 @@ Definition wrapper_step (prog : progC) : mrel (exprW * stateW) (exprW * stateW) 
            χC ρc' = χC ρc →
            rootsC ρc' = rootsC ρc →
            privσC ρc' = privσC ρc →
-           φ (RunningW (fillC K (of_val_C a)), C (ρc', mem')))
+           φ (WrapExprC (language.fill K (C_lang.of_val (LitV (LitLoc a)))), C (ρc', mem')))
     ∨
     (* call to "registerroot" *)
-    (∀ K ec w ρc mem,
-       e = RunningW (fillC K ec) →
-       to_call_C ec = Some ("registerroot", [w]) →
+    (∀ K ec a ρc mem,
+       e = WrapExprC (language.fill K ec) →
+       to_call ec = Some ("registerroot", [LitV (LitLoc a)]) →
        ρ = C (ρc, mem) →
-       w ∉ rootsC ρc →
+       a ∉ rootsC ρc →
        ∀ ρc',
-         rootsC ρc' = {[ w ]} ∪ rootsC ρc →
+         rootsC ρc' = {[ a ]} ∪ rootsC ρc →
          χC ρc' = χC ρc →
          ζC ρc' = ζC ρc →
          θC ρc' = θC ρc →
          privσC ρc' = privσC ρc →
-         φ (RunningW (fillC K (of_val_C 0%Z)), C (ρc', mem)))
+         φ (WrapExprC (language.fill K (C_lang.of_val (LitV (LitInt 0)))), C (ρc', mem)))
     ∨
     (* call to "unregisterroot" *)
-    (∀ K ec w ρc mem,
-       e = RunningW (fillC K ec) →
-       to_call_C ec = Some ("unregisterroot", [w]) →
+    (∀ K ec a ρc mem,
+       e = WrapExprC (language.fill K ec) →
+       to_call ec = Some ("unregisterroot", [LitV (LitLoc a)]) →
        ρ = C (ρc, mem) →
-       w ∈ rootsC ρc →
+       a ∈ rootsC ρc →
        ∀ ρc',
-         rootsC ρc' = rootsC ρc ∖ {[ w ]} →
+         rootsC ρc' = rootsC ρc ∖ {[ a ]} →
          χC ρc' = χC ρc →
          ζC ρc' = ζC ρc →
          θC ρc' = θC ρc →
          privσC ρc' = privσC ρc →
-         φ (RunningW (fillC K (of_val_C 0%Z)), C (ρc', mem)))
+         φ (WrapExprC (language.fill K (C_lang.of_val (LitV (LitInt 0)))), C (ρc', mem)))
     ∨
     (* call to "modify" *)
     (∀ K ec w i w' ρc mem γ lv blk blk',
-       e = RunningW (fillC K ec) →
-       to_call_C ec = Some ("modify", [w; i; w']) →
+       e = WrapExprC (language.fill K ec) →
+       to_call ec = Some ("modify", [w; LitV (LitInt i); w']) →
        ρ = C (ρc, mem) →
        (0 ≤ i)%Z →
        repr_lval (θC ρc) (Lloc γ) w →
@@ -152,38 +192,38 @@ Definition wrapper_step (prog : progC) : mrel (exprW * stateW) (exprW * stateW) 
          θC ρc' = θC ρc →
          rootsC ρc' = rootsC ρc →
          privσC ρc' = privσC ρc →
-         φ (RunningW (fillC K (of_val_C 0%Z)), C (ρc', mem)))
+         φ (WrapExprC (language.fill K (C_lang.of_val (LitV (LitInt 0)))), C (ρc', mem)))
     ∨
     (* call to "readfield" *)
     (∀ K ec w i ρc mem γ mut tag lvs lv w',
-       e = RunningW (fillC K ec) →
-       to_call_C ec = Some ("readfield", [w; i]) →
+       e = WrapExprC (language.fill K ec) →
+       to_call ec = Some ("readfield", [w; LitV (LitInt i)]) →
        ρ = C (ρc, mem) →
        (0 ≤ i)%Z →
        repr_lval (θC ρc) (Lloc γ) w →
        (ζC ρc) !! γ = Some (mut, tag, lvs) →
        lvs !! (Z.to_nat i) = Some lv →
        repr_lval (θC ρc) lv w' →
-       φ (RunningW (fillC K (of_val_C w')), C (ρc, mem)))
+       φ (WrapExprC (language.fill K (C_lang.of_val w')), C (ρc, mem)))
     ∨
     (* call to "val2int" *)
-    (∀ K ec ρc mem w w',
-       e = RunningW (fillC K ec) →
-       to_call_C ec = Some ("val2int", [w]) →
+    (∀ K ec ρc mem w x,
+       e = WrapExprC (language.fill K ec) →
+       to_call ec = Some ("val2int", [w]) →
        ρ = C (ρc, mem) →
-       repr_lval (θC ρc) (Lint w') w →
-       φ (RunningW (fillC K (of_val_C w')), (C (ρc, mem))))
+       repr_lval (θC ρc) (Lint x) w →
+       φ (WrapExprC (language.fill K (C_lang.of_val (LitV (LitInt x)))), (C (ρc, mem))))
     ∨
     (* call to "int2val" *)
-    (∀ K ec ρc mem w w',
-       e = RunningW (fillC K ec) →
-       to_call_C ec = Some ("int2val", [w]) →
+    (∀ K ec ρc mem x w,
+       e = WrapExprC (language.fill K ec) →
+       to_call ec = Some ("int2val", [LitV (LitInt x)]) →
        ρ = C (ρc, mem) →
-       repr_lval (θC ρc) (Lint w) w' →
-       φ (RunningW (fillC K (of_val_C w')), (C (ρc, mem)))).
+       repr_lval (θC ρc) (Lint x) w →
+       φ (WrapExprC (language.fill K (C_lang.of_val w)), (C (ρc, mem)))).
 
-Program Definition wrapper_step_umrel (p : progC) : umrel (exprW * stateW) (exprW * stateW) :=
-  {| rel := wrapper_step p |}.
+Program Definition wrapper_step_umrel (P : prog) : umrel (expr * state) (expr * state) :=
+  {| rel := wrapper_step P |}.
 Next Obligation.
   unfold upclosed. intros p [e ρ] φ ψ H Hφψ.
   destruct_or! H; naive_solver.
