theories/interop/assums.v
@@ -10,9 +10,11 @@ From stdpp Require Import base gmap.
 
 (* toyML *)
 
+Module ML_lang.
+
 Parameter loc : Set.
 Context `{EqDecision loc, Countable loc}.
-Parameter exprML : Type.
+Parameter expr : Type.
 
 Inductive base_lit : Set :=
   | LitInt (n : Z) | LitBool (b : bool) | LitUnit
@@ -20,7 +22,7 @@ Inductive base_lit : Set :=
 
 Inductive val :=
   | LitV (l : base_lit)
-  | RecV (f x : binder) (e : exprML)
+  | RecV (f x : binder) (e : expr)
   | PairV (v1 v2 : val)
   | InjLV (v : val)
   | InjRV (v : val).
@@ -29,23 +31,8 @@ Definition store : Type := gmap loc (list val).
 Implicit Type ℓ : loc.
 Implicit Type σ : store.
 
-Parameter progML : Type.
-Parameter ectxML : Type.
-Parameter head_step_ML : progML → exprML → store → exprML → store → Prop.
+Parameter prog : Type.
+Parameter ectx : Type.
+Parameter head_step : prog → expr → store → expr → store → Prop.
 
-(* toyC *)
-
-Definition addr : Type := Z.
-Definition word : Type := Z.
-Definition memory : Type := gmap addr word.
-
-Parameter exprC : Type.
-Definition progC : Type := gmap string (list string * exprC).
-Parameter ectxC : Type.
-Parameter head_step_C : progC → exprC → memory → exprC → memory → Prop.
-Parameter exprC_of_call : string → list word → exprC.
-Parameter fillC : ectxC → exprC → exprC.
-Parameter apply_func_C : string → list word → exprC.
-Parameter to_val_C : exprC → option word.
-Parameter to_call_C : exprC → option (string * list word).
-Parameter of_val_C : word → exprC.
+End ML_lang.
